Reorganisation

proofs/LabeledGraphSemantics.thy
@@ -13,13 +13,6 @@ datatype 'v allegorical_term
  | A_Cnv "'v allegorical_term"
  | A_Lbl (a_lbl : 'v)
 
-datatype 'v Standard_Constant = S_Top | S_Bot | S_Idt | S_Const 'v
-
-abbreviation "a_bot \<equiv> A_Lbl S_Bot"
-abbreviation "a_top \<equiv> A_Lbl S_Top"
-notation a_bot ("\<bottom>")
-notation a_top ("\<top>")
-
 fun semantics where
 "semantics G (A_Int a b) = semantics G a \<inter> semantics G b" |
 "semantics G (A_Cmp a b) = semantics G a O semantics G b" |
@@ -29,9 +22,8 @@ fun semantics where
 notation semantics (":_:\<lbrakk>_\<rbrakk>" 55)
 
 type_synonym 'v sentence = "'v allegorical_term \<times> 'v allegorical_term"
-type_synonym 'v std_term = "'v Standard_Constant allegorical_term"
-type_synonym 'v std_sentence = "'v std_term \<times> 'v std_term"
-type_synonym 'v std_graph = "('v Standard_Constant, 'v Standard_Constant) labeled_graph"
+
+datatype 'v Standard_Constant = S_Top | S_Bot | S_Idt | S_Const 'v
 
 abbreviation holds where
 "holds G S \<equiv> :G:\<lbrakk>fst S\<rbrakk> = :G:\<lbrakk>snd S\<rbrakk>"
@@ -47,38 +39,6 @@ lemma sentence_iff: (* Lemma 1 *)
   "G \<tturnstile> (e\<^sub>1, e\<^sub>2) = (G \<tturnstile> e\<^sub>1 \<sqsubseteq> e\<^sub>2 \<and> G \<tturnstile> e\<^sub>2 \<sqsubseteq> e\<^sub>1)"
   by auto
 
-definition standard :: "'l set \<Rightarrow> 'l \<Rightarrow> 'l \<Rightarrow> 'l \<Rightarrow> ('l, 'l) labeled_graph \<Rightarrow> bool" where
-"standard C b t idt G
-   \<equiv> G = restrict G
-   \<and> vertices G \<noteq> {}
-   \<and> getRel idt G = {(x,x). x\<in>vertices G}
-   \<and> getRel b G = {}
-   \<and> getRel t G = {(x,y). x\<in>vertices G \<and> y\<in>vertices G}
-   \<and> (\<forall> c \<in> C. getRel c G = {(c,c)})"
 
-abbreviation standard' :: "'a std_graph \<Rightarrow> bool" where
-"standard' \<equiv> standard (S_Const ` UNIV) S_Bot S_Top S_Idt"
-
-definition model :: "'a std_graph \<Rightarrow> ('a std_sentence) set \<Rightarrow> bool" where
-"model G T \<equiv> standard' G \<and> (\<forall> S \<in> T. G \<tturnstile> S)"
-notation model (infix "\<tturnstile>\<^sub>S" 55) (* S for standard *)
-
-abbreviation consistent :: "('a std_sentence) set \<Rightarrow> bool" where
-"consistent T \<equiv> \<exists> G. model G T"
-
-definition entails where
-"entails T S \<equiv> \<forall> G. G \<tturnstile>\<^sub>S T \<longrightarrow> G \<tturnstile> S"
-
-lemma standard_top_not_bot[intro]:
-"standard' G \<Longrightarrow> :G:\<lbrakk>\<bottom>\<rbrakk> \<noteq> :G:\<lbrakk>\<top>\<rbrakk>"
-  unfolding standard_def by auto
-
-lemma consistent_iff_entails_nonsense: (* Lemma 2 *)
-"consistent T = (\<not> entails T (\<bottom>,\<top>))"
-proof
-  show "consistent T \<Longrightarrow> \<not> entails T (\<bottom>, \<top>)"
-    using standard_top_not_bot unfolding entails_def model_def
-    by fastforce
-qed (auto simp:entails_def model_def)
 
 end
