proofs/RuleSemanticsConnection.thy
@@ -2,23 +2,7 @@ theory RuleSemanticsConnection
 imports LabeledGraphSemantics RulesAndChains
 begin
 
-(* gets the top relation-label as argument *)
-definition top_rule :: "'l \<Rightarrow> ('l,'v::{one,zero,numeral}) Graph_PreRule" where
-"top_rule t = (LG {} {0,1},LG {(t,0,1)} {0,1})"
-
-definition nonempty_rule :: "('l,'v::{one,zero,numeral}) Graph_PreRule" where
-"nonempty_rule = (LG {} {},LG {} {0})"
-
-(* gets a reflexive relation-label as argument *)
-definition reflexivity_rule :: "'l \<Rightarrow> ('l,'v::{one,zero,numeral}) Graph_PreRule" where
-"reflexivity_rule t = (LG {} {0},LG {(t,0,0)} {0})"
-
-lemma are_rules[intro]:
-"graph_rule nonempty_rule"
-"graph_rule (top_rule t)"
-"graph_rule (reflexivity_rule i)"
-  unfolding reflexivity_rule_def top_rule_def nonempty_rule_def is_graph_homomorphism_def
-  by auto
+(* File contains Definition 15, Lemma 5 and Lemma 6 *)
 
 fun translation :: "'c allegorical_term \<Rightarrow> ('c, nat) labeled_graph" where
 "translation (A_Lbl l) = LG {(l,0,1)} {0,1}" |
@@ -478,5 +462,5 @@ proof
   }
   thus ?lhs by auto
 qed
-(* Work towards Lemma 6 and 7 *)
+
 end
