proofs/StandardModels.thy
@@ -1,0 +1,48 @@
+theory StandardModels
+imports LabeledGraphSemantics
+begin
+
+abbreviation "a_bot \<equiv> A_Lbl S_Bot"
+abbreviation "a_top \<equiv> A_Lbl S_Top"
+notation a_bot ("\<bottom>")
+notation a_top ("\<top>")
+
+type_synonym 'v std_term = "'v Standard_Constant allegorical_term"
+type_synonym 'v std_sentence = "'v std_term \<times> 'v std_term"
+type_synonym 'v std_graph = "('v Standard_Constant, 'v Standard_Constant) labeled_graph"
+
+definition standard :: "'l set \<Rightarrow> 'l \<Rightarrow> 'l \<Rightarrow> 'l \<Rightarrow> ('l, 'l) labeled_graph \<Rightarrow> bool" where
+"standard C b t idt G
+   \<equiv> G = restrict G
+   \<and> vertices G \<noteq> {}
+   \<and> getRel idt G = {(x,x). x\<in>vertices G}
+   \<and> getRel b G = {}
+   \<and> getRel t G = {(x,y). x\<in>vertices G \<and> y\<in>vertices G}
+   \<and> (\<forall> c \<in> C. getRel c G = {(c,c)})"
+
+abbreviation standard' :: "'a std_graph \<Rightarrow> bool" where
+"standard' \<equiv> standard (S_Const ` UNIV) S_Bot S_Top S_Idt"
+
+definition model :: "'a std_graph \<Rightarrow> ('a std_sentence) set \<Rightarrow> bool" where
+"model G T \<equiv> standard' G \<and> (\<forall> S \<in> T. G \<tturnstile> S)"
+notation model (infix "\<tturnstile>\<^sub>S" 55) (* S for standard *)
+
+abbreviation consistent :: "('a std_sentence) set \<Rightarrow> bool" where
+"consistent T \<equiv> \<exists> G. model G T"
+
+definition entails where
+"entails T S \<equiv> \<forall> G. G \<tturnstile>\<^sub>S T \<longrightarrow> G \<tturnstile> S"
+
+lemma standard_top_not_bot[intro]:
+"standard' G \<Longrightarrow> :G:\<lbrakk>\<bottom>\<rbrakk> \<noteq> :G:\<lbrakk>\<top>\<rbrakk>"
+  unfolding standard_def by auto
+
+lemma consistent_iff_entails_nonsense: (* Lemma 2 *)
+"consistent T = (\<not> entails T (\<bottom>,\<top>))"
+proof
+  show "consistent T \<Longrightarrow> \<not> entails T (\<bottom>, \<top>)"
+    using standard_top_not_bot unfolding entails_def model_def
+    by fastforce
+qed (auto simp:entails_def model_def)
+
+end
