proofs/StandardRules.thy
@@ -1,0 +1,10 @@
+theory StandardRules
+imports StandardModels RuleSemanticsConnection
+begin
+
+
+(* Definitions 16 to 20 *)
+
+(* Work towards Lemma 7 and 8 *)
+
+end
